rustfrontend/RustIRsem.v
@@ -366,7 +366,7 @@ Inductive step : state -> trace -> state -> Prop :=
     (* there is no receiver for the moved place, so it must be None *)
     eval_expr ge e m ge a v1 ->
     to_ctype (typeof a) = ty ->
-    bool_val v1 ty m = Some b ->
+    Cop.bool_val v1 ty m = Some b ->
     step (State f (Sifthenelse a s1 s2) k e m)
       E0 (State f (if b then s1 else s2) k e m)
 | step_loop: forall f s k e m,
